cedar-lean/Cedar/Thm/TPE.lean
@@ -46,56 +46,141 @@ theorem partialEvaluate_is_sound
   intro h₀ h₁ h₂ h₃
   cases x
   case and x₁ x₂ ty =>
-    sorry
+    cases h₀
+    rename_i h₄ h₅ h₆ _
+    have hᵢ₁ := partialEvaluate_is_sound h₄ h₁ h₂ h₃
+    rcases h₆ with ⟨h₆₁, h₆₂⟩
+    simp [TypedExpr.toExpr, Spec.evaluate]
+    generalize hᵢ₁₁ : Spec.evaluate x₁.toExpr req₁ es₁ = res₁
+    cases res₁
+    case _ =>
+      rcases to_option_left_err hᵢ₁ hᵢ₁₁ with ⟨_, hᵢ₁₂⟩
+      simp [Result.as, TPE.evaluate]
+      -- essentially (TPE.evaluate x₁ req₂ es₂).evaluate req₁ es₁ = .error _ → (TPE.and (TPE.evaluate x₁ req₂ es₂) (TPE.evaluate x₂ req₂ es₂) ty).evaluate req₁ es₁) = .error _
+      sorry
+    case _ v₁ =>
+      rcases well_typed_bool h₁ h₄ h₆₁ hᵢ₁₁ with ⟨b₁, hᵢ₁₁'⟩
+      have hᵢ₁₂ := to_option_left_ok hᵢ₁ hᵢ₁₁
+      simp [hᵢ₁₁', Result.as, Coe.coe, Value.asBool, TPE.evaluate, TPE.and]
+      split <;> split
+      · rename_i hb _ _ _ _ _ heq _
+        simp [heq, Residual.evaluate, hᵢ₁₁', hb] at hᵢ₁₂
+      · rename_i hb _ _ _ _ _ _ _
+        simp [Residual.evaluate, hb]
+      · rename_i heq _
+        simp [heq, Residual.evaluate] at hᵢ₁₂
+      · simp [hᵢ₁₂, hᵢ₁₁']
+      · rename_i hb _ _ _ _ _ _ _ _ _
+        simp [Residual.evaluate, hᵢ₁₂, hᵢ₁₁', hb, Result.as, Coe.coe, Value.asBool]
+      · rename_i hb _ v₂ heq
+        simp at hb
+        rcases well_typed_bool h₁ h₅ h₆₂ heq with ⟨b₂, hᵢ₂⟩
+        split
+        · simp
+          sorry
+        · rename_i heq₁
+          simp [hᵢ₂] at heq₁
+      · rename_i heq
+        sorry
   case lit => sorry
   case var => sorry
   case ite cond thenExpr elseExpr ty =>
     cases h₀
-    rename_i h₄ h₅ h₆ h₇ h₈
+    rename_i h₄ h₅ h₆ h₇ _
     simp [TypedExpr.toExpr, Spec.evaluate]
     generalize hᵢ₁ : Spec.evaluate cond.toExpr req₁ es₁ = res₁
     cases res₁
     case _ =>
       sorry
     case _ v₁ =>
-      have hᵢ₁' := typechecked_is_well_typed h₁ h₄ hᵢ₁
-      simp [CedarType.isBool] at h₅
-      split at h₅
-      · rename_i heq
-        simp only [heq] at hᵢ₁'
-        have ⟨b, hᵢ₁'⟩ := instance_of_bool_is_bool hᵢ₁'
-        simp [hᵢ₁', Result.as, Coe.coe, Value.asBool]
-        have hᵢ₁₁ : (TPE.evaluate cond req₂ es₂).evaluate req₁ es₁ = .ok v₁
-        := by sorry
-        simp [TPE.evaluate, TPE.ite]
-        split <;> split
-        · rename_i  hb _ _ _ heq₁
-          simp [heq₁, Residual.evaluate, hᵢ₁', hb] at hᵢ₁₁
-          simp [hᵢ₁₁]
-          exact partialEvaluate_is_sound h₆ h₁ h₂ h₃
-        · rename_i heq₁
-          simp [heq₁, Residual.evaluate] at hᵢ₁₁
-        · rename_i hb _ _ _
-          simp [Residual.evaluate, hᵢ₁₁, hᵢ₁', hb, Value.asBool]
-          exact partialEvaluate_is_sound h₆ h₁ h₂ h₃
-        · rename_i hb _ _ _ heq₁
-          simp at hb
-          simp [heq₁, Residual.evaluate, hᵢ₁', hb] at hᵢ₁₁
-          simp [hᵢ₁₁]
-          exact partialEvaluate_is_sound h₇ h₁ h₂ h₃
-        · rename_i heq₁
-          simp [heq₁, Residual.evaluate] at hᵢ₁₁
-        · rename_i hb _ _ _
-          simp at hb
-          simp [hb] at hᵢ₁'
-          simp [hᵢ₁'] at hᵢ₁₁
-          simp [Residual.evaluate, hᵢ₁₁, Value.asBool]
-          exact partialEvaluate_is_sound h₇ h₁ h₂ h₃
+      rcases well_typed_bool h₁ h₄ h₅ hᵢ₁ with ⟨b₁, hᵢ₁'⟩
+      simp [hᵢ₁', Result.as, Coe.coe, Value.asBool]
+      have hᵢ₁₁ : (TPE.evaluate cond req₂ es₂).evaluate req₁ es₁ = .ok v₁
+      := by sorry
+      simp [TPE.evaluate, TPE.ite]
+      split <;> split
+      · rename_i  hb _ _ _ heq₁
+        simp [heq₁, Residual.evaluate, hᵢ₁', hb] at hᵢ₁₁
+        simp [hᵢ₁₁]
+        exact partialEvaluate_is_sound h₆ h₁ h₂ h₃
+      · rename_i heq₁
+        simp [heq₁, Residual.evaluate] at hᵢ₁₁
+      · rename_i hb _ _ _
+        simp [Residual.evaluate, hᵢ₁₁, hᵢ₁', hb, Value.asBool]
+        exact partialEvaluate_is_sound h₆ h₁ h₂ h₃
+      · rename_i hb _ _ _ heq₁
+        simp at hb
+        simp [heq₁, Residual.evaluate, hᵢ₁', hb] at hᵢ₁₁
+        simp [hᵢ₁₁]
+        exact partialEvaluate_is_sound h₇ h₁ h₂ h₃
+      · rename_i heq₁
+        simp [heq₁, Residual.evaluate] at hᵢ₁₁
+      · rename_i hb _ _ _
+        simp at hb
+        simp [hb] at hᵢ₁'
+        simp [hᵢ₁'] at hᵢ₁₁
+        simp [Residual.evaluate, hᵢ₁₁, Value.asBool]
+        exact partialEvaluate_is_sound h₇ h₁ h₂ h₃
   case or => sorry
   case unaryApp => sorry
   case binaryApp => sorry
   case getAttr => sorry
-  case hasAttr => sorry
+  case hasAttr x₁ attr ty =>
+    cases h₀
+    rename_i h₄ h₅ h₆
+    have hᵢ₁ := partialEvaluate_is_sound h₄ h₁ h₂ h₃
+    generalize hᵢ₁₁ : Spec.evaluate x₁.toExpr req₁ es₁ = res₁
+    cases res₁
+    case _ =>
+      rcases to_option_left_err hᵢ₁ hᵢ₁₁ with ⟨_, hᵢ₁₂⟩
+      simp [TypedExpr.toExpr, Spec.evaluate, hᵢ₁₁, TPE.evaluate, TPE.hasAttr]
+      split
+      · simp [Residual.evaluate, Except.toOption]
+      · split
+        · rename_i heq
+          simp [TPE.attrsOf] at heq
+          split at heq
+          · rename_i heq₁
+            simp [heq₁, Residual.evaluate] at hᵢ₁₂
+          · rename_i heq₁
+            simp [heq₁, Residual.evaluate] at hᵢ₁₂
+          · cases heq
+        · rename_i heq
+          simp [TPE.attrsOf] at heq
+          split at heq
+          · cases heq
+          · rename_i heq₁
+            simp [heq₁, Residual.evaluate] at hᵢ₁₂
+          · simp [Residual.evaluate, hᵢ₁₂, Except.toOption]
+    case _ v =>
+      simp [TypedExpr.toExpr, Spec.evaluate, hᵢ₁₁, Spec.hasAttr, Spec.attrsOf]
+      cases h₅
+      case _ hₜ =>
+        sorry
+      case _ hₜ =>
+        have ⟨m, hᵢ₁₂⟩ := well_typed_record h₁ h₄ hₜ hᵢ₁₁
+        simp [hᵢ₁₂]
+        have hᵢ₁₂' := to_option_left_ok hᵢ₁ hᵢ₁₁
+        simp [TPE.evaluate, TPE.hasAttr]
+        split
+        · rename_i heq
+          simp [heq, Residual.evaluate] at hᵢ₁₂'
+        · split <;> rename_i heq₁ <;> simp [TPE.attrsOf] at heq₁
+          · split at heq₁
+            · rename_i heq₂
+              simp [heq₂, Residual.evaluate] at hᵢ₁₂'
+              simp at heq₁
+              simp [hᵢ₁₂] at hᵢ₁₂'
+              simp [←heq₁, Residual.evaluate, hᵢ₁₂']
+            · rename_i heq₂
+              simp [heq₂, Residual.evaluate, hᵢ₁₂] at hᵢ₁₂'
+            · cases heq₁
+          · split at heq₁
+            · cases heq₁
+            · rename_i heq₂
+              simp [heq₂, Residual.evaluate] at hᵢ₁₂'
+              simp [hᵢ₁₂] at hᵢ₁₂'
+            · simp [Residual.evaluate, hᵢ₁₂', hᵢ₁₂, Spec.hasAttr, Spec.attrsOf]
   case set => sorry
   case record => sorry
   case call => sorry
